ocaml/src/TypeUtil.ml
@@ -16,26 +16,13 @@
 
 open Util
 open ConfigUtil
+open DataUtil
 open Compiler.EnhancedCompiler
 
 (* Data utils for the Camp evaluator and compiler *)
 
-type io_hierarchy = Data.json
-type io_json = Data.json option
-
-type io_hierarchy_list = (string * string) list
-type io_input = Data.data list
-type io_output = Data.data list
-
-type rtype_content = Data.json
-type model_content = string * (string * string) list * (string * rtype_content) list
-      
-val get_io_content : io_json -> Data.json * Data.json * Data.json * Data.json * Data.json
-val get_hierarchy : io_json -> io_hierarchy
-val get_hierarchy_cloudant : io_json -> io_hierarchy
-val build_hierarchy : io_hierarchy -> io_hierarchy_list
-val get_input : ConfigUtil.eval_config -> io_json -> io_input
-val get_output : io_json -> io_output
-
-val get_model_content : Data.json -> model_content
+let rtype_content_to_rtype (br: (string * string) list) (j:rtype_content) =
+  match RType.json_to_rtype_with_fail (List.map (fun xy -> (Util.char_list_of_string (fst xy), Util.char_list_of_string (snd xy))) br) j with
+  | None -> raise (Failure ("type parsing failed for JSON:" ^ (Util.string_of_char_list (Data.jsonToJS ['"'] j))))
+  | Some t -> t
 
