coq/Compiler/CompilerModel/TrivialModel.v
@@ -15,7 +15,7 @@
  *)
 
 Require Import Utils BasicSystem.
-Require Import ForeignToJava ForeignToJavascript ForeignToJSON.
+Require Import ForeignToJava ForeignToJavascript ForeignToJSON ForeignTypeToJSON.
 Require Import ForeignReduceOps ForeignToReduceOps.
 Require Import ForeignToSpark.
 Require Import ForeignCloudant ForeignToCloudant.
@@ -239,6 +239,15 @@ Defined.
      destruct fd. 
   Defined.
 
+  Program Instance trivial_foreign_type_to_JSON : foreign_type_to_JSON
+    := mk_foreign_type_to_JSON trivial_foreign_type _ _.
+  Next Obligation.
+    exact None.
+  Defined.
+  Next Obligation.
+     destruct fd. 
+  Defined.
+
   Program Instance trivial_foreign_reduce_op
             {fdata:foreign_data}:
       foreign_reduce_op
@@ -299,6 +308,8 @@ Existing Instance silent_optimizer_logger.
       := trivial_foreign_to_javascript.
     Definition compiler_foreign_to_JSON : foreign_to_JSON
       := trivial_foreign_to_JSON.
+    Definition compiler_foreign_type_to_JSON : foreign_type_to_JSON
+      := trivial_foreign_type_to_JSON.
     Definition compiler_foreign_reduce_op : foreign_reduce_op
       := trivial_foreign_reduce_op.
     Definition compiler_foreign_to_reduce_op : foreign_to_reduce_op
@@ -334,6 +345,8 @@ Existing Instance silent_optimizer_logger.
       := trivial_foreign_to_javascript.
     Definition compiler_model_foreign_to_JSON : foreign_to_JSON
       := trivial_foreign_to_JSON.
+    Definition compiler_model_foreign_type_to_JSON : foreign_type_to_JSON
+      := trivial_foreign_type_to_JSON.
     Definition compiler_model_foreign_reduce_op : foreign_reduce_op
       := trivial_foreign_reduce_op.
     Definition compiler_model_foreign_to_reduce_op : foreign_to_reduce_op
